Coq/Cln/RepComp/Cln_Rigidity_Interface.v
@@ -1,3 +1,0 @@
-(*
-Your axiomatized hard family / LB, but now phrased in terms of GAProg size.
-*)
